Finish translating Katovsky's first theory about categories
(there are six more in his Isabelle development)
This includes definition of category, various theorems about
isomorphisms and inverses, and examples of the unit category and the
opposite category.

examples/category/categoryScript.sml
@@ -1,17 +1,18 @@
-open HolKernel boolLib bossLib
+open HolKernel boolLib bossLib lcsymtacs SatisfySimps
 
 val _ = new_theory "category"
 
 val extensional_def = Define`
-  extensional f x = !e. e NOTIN x ==> (f e = ARB)`
+  extensional f x = ∀e. e ∉ x ⇒ (f e = ARB)`
 
 val restrict_def = Define`
-  restrict f x = \e. if e IN x then f e else ARB`
+  restrict f x = λe. if e ∈ x then f e else ARB`
 
 val extensional_restrict = Q.store_thm(
 "extensional_restrict",
-`extensional (restrict f x) x`,
-SRW_TAC [][extensional_def,restrict_def])
+`∀f x. extensional (restrict f x) x`,
+srw_tac [][extensional_def,restrict_def])
+val _ = export_rewrites["extensional_restrict"]
 
 val _ = Hol_datatype `category =
   <| obj : 'a set ;
@@ -20,35 +21,36 @@ val _ = Hol_datatype `category =
      cod : 'b -> 'a ;
      id : 'a -> 'b ;
      comp : 'b # 'b -> 'b |>`
+val category_component_equality = DB.theorem "category_component_equality"
 
 val maps_to_def = Define`
-  maps_to c f x y = f IN c.mor /\ (c.dom f = x) /\ (c.cod f = y)`
+  maps_to c f x y = f ∈ c.mor ∧ (c.dom f = x) ∧ (c.cod f = y)`
 
 val composable_def = Define`
-  composable c gf = (SND gf) IN c.mor /\ (FST gf) IN c.mor /\
+  composable c gf = (SND gf) IN c.mor ∧ (FST gf) IN c.mor ∧
                     (c.cod (SND gf) = c.dom (FST gf))`
 
 val extensional_category_def = Define`
   extensional_category c =
-    extensional c.dom c.mor /\
-    extensional c.cod c.mor /\
-    extensional c.id c.obj /\
+    extensional c.dom c.mor ∧
+    extensional c.cod c.mor ∧
+    extensional c.id c.obj ∧
     extensional c.comp (composable c)`
 
 val category_axioms_def = Define`
   category_axioms c =
-    (!f. f IN c.mor ==> c.dom f IN c.obj) /\
-    (!f. f IN c.mor ==> c.cod f IN c.obj) /\
-    (!a. a IN c.obj ==> maps_to c (c.id a) a a) /\
-    (!f. f IN c.mor ==> (c.comp (f, c.id (c.dom f)) = f)) /\
-    (!f. f IN c.mor ==> (c.comp (c.id (c.cod f), f) = f)) /\
-    (!f g h. composable c (g,f) /\ composable c (h,g) ==>
-             (c.comp (h, (c.comp (g,f))) = c.comp (c.comp (h,g), f))) /\
-    (!f g x y z. maps_to c f x y /\ maps_to c g y z ==>
+    (∀f. f ∈ c.mor ⇒ c.dom f ∈ c.obj) ∧
+    (∀f. f ∈ c.mor ⇒ c.cod f ∈ c.obj) ∧
+    (∀a. a ∈ c.obj ⇒ maps_to c (c.id a) a a) ∧
+    (∀f. f ∈ c.mor ⇒ (c.comp (f, c.id (c.dom f)) = f)) ∧
+    (∀f. f ∈ c.mor ⇒ (c.comp (c.id (c.cod f), f) = f)) ∧
+    (∀f g h. composable c (g,f) ∧ composable c (h,g) ⇒
+             (c.comp (h, (c.comp (g,f))) = c.comp (c.comp (h,g), f))) ∧
+    (∀f g x y z. maps_to c f x y ∧ maps_to c g y z ⇒
                  maps_to c (c.comp (g,f)) x z)`
 
 val is_category_def = Define`
-  is_category c = extensional_category c /\ category_axioms c`
+  is_category c = extensional_category c ∧ category_axioms c`
 
 val mk_cat_def = Define`
   mk_cat (c:('a,'b) category) = <|
@@ -61,88 +63,422 @@ val mk_cat_def = Define`
 
 val mk_cat_maps_to = Q.store_thm(
 "mk_cat_maps_to",
-`maps_to (mk_cat c) f x y = maps_to c f x y`,
-SRW_TAC [][maps_to_def,mk_cat_def,restrict_def])
+`∀c f x y. maps_to (mk_cat c) f x y = maps_to c f x y`,
+srw_tac [][maps_to_def,mk_cat_def,restrict_def])
 
 val mk_cat_composable = Q.store_thm(
 "mk_cat_composable",
-`composable (mk_cat c) gf = composable c gf`,
-SRW_TAC [][composable_def,mk_cat_def,restrict_def])
+`∀c gf. composable (mk_cat c) gf = composable c gf`,
+srw_tac [][composable_def,mk_cat_def,restrict_def])
 
 val mk_cat_id = Q.store_thm(
 "mk_cat_id",
-`a IN c.obj ==> ((mk_cat c).id a = c.id a)`,
-SRW_TAC [][mk_cat_def,restrict_def])
+`∀c a. a ∈ c.obj ⇒ ((mk_cat c).id a = c.id a)`,
+srw_tac [][mk_cat_def,restrict_def])
 
 val mk_cat_obj = Q.store_thm(
 "mk_cat_obj",
-`(mk_cat c).obj = c.obj`,
-SRW_TAC [][mk_cat_def])
+`∀c. (mk_cat c).obj = c.obj`,
+srw_tac [][mk_cat_def])
 
 val mk_cat_mor = Q.store_thm(
-"mk_cat_obj",
-`(mk_cat c).mor = c.mor`,
-SRW_TAC [][mk_cat_def])
+"mk_cat_mor",
+`∀c. (mk_cat c).mor = c.mor`,
+srw_tac [][mk_cat_def])
 
 val mk_cat_dom = Q.store_thm(
 "mk_cat_dom",
-`f IN c.mor ==> ((mk_cat c).dom f = c.dom f)`,
-SRW_TAC [][mk_cat_def,restrict_def])
+`∀c f. f ∈ c.mor ⇒ ((mk_cat c).dom f = c.dom f)`,
+srw_tac [][mk_cat_def,restrict_def])
 
 val mk_cat_cod = Q.store_thm(
 "mk_cat_cod",
-`f IN c.mor ==> ((mk_cat c).cod f = c.cod f)`,
-SRW_TAC [][mk_cat_def,restrict_def])
+`∀c f. f ∈ c.mor ⇒ ((mk_cat c).cod f = c.cod f)`,
+srw_tac [][mk_cat_def,restrict_def])
+
+val _ = export_rewrites
+["mk_cat_maps_to","mk_cat_composable",
+ "mk_cat_id","mk_cat_obj","mk_cat_mor",
+ "mk_cat_dom","mk_cat_cod"]
 
 val mk_cat_composable = Q.store_thm(
 "mk_cat_composable",
-`composable (mk_cat c) = composable c `,
-SRW_TAC [][FUN_EQ_THM] THEN
-METIS_TAC [composable_def,mk_cat_cod,mk_cat_dom,mk_cat_mor])
+`∀c. composable (mk_cat c) = composable c `,
+srw_tac [][FUN_EQ_THM,composable_def])
 
 val mk_cat_comp = Q.store_thm(
 "mk_cat_comp",
-`composable c gf ==> ((mk_cat c).comp gf = c.comp gf)`,
-SRW_TAC [][mk_cat_def,restrict_def,IN_DEF])
+`∀c gf. composable c gf ⇒ ((mk_cat c).comp gf = c.comp gf)`,
+srw_tac [][mk_cat_def,restrict_def,IN_DEF])
+
+val _ = export_rewrites["mk_cat_composable","mk_cat_comp"]
 
 val extensional_mk_cat = Q.store_thm(
 "extensional_mk_cat",
-`extensional_category (mk_cat c)`,
-SRW_TAC [][extensional_category_def]
-THEN1 SRW_TAC [][mk_cat_def,extensional_restrict]
-THEN1 SRW_TAC [][mk_cat_def,extensional_restrict]
-THEN1 SRW_TAC [][mk_cat_def,extensional_restrict] THEN
-SRW_TAC [][Once mk_cat_def,mk_cat_composable,extensional_restrict])
+`∀c. extensional_category (mk_cat c)`,
+srw_tac [][extensional_category_def,mk_cat_def])
+val _ = export_rewrites["extensional_mk_cat"]
+
+val maps_to_dom_composable = Q.store_thm(
+"maps_to_dom_composable",
+`∀c gf x. (FST gf) ∈ c.mor ∧ maps_to c (SND gf) x (c.dom (FST gf)) ⇒ composable c gf`,
+srw_tac [][composable_def,maps_to_def])
+
+val maps_to_cod_composable = Q.store_thm(
+"maps_to_cod_composable",
+`∀c gf y. (SND gf) ∈ c.mor ∧ maps_to c (FST gf) (c.cod (SND gf)) y ⇒ composable c gf`,
+srw_tac [][composable_def,maps_to_def])
 
 val mk_cat_is_category = Q.store_thm(
 "mk_cat_is_category",
-`category_axioms c ==> is_category (mk_cat c)`,
-SRW_TAC [][is_category_def,extensional_mk_cat] THEN
-FULL_SIMP_TAC (srw_ss()) [category_axioms_def] THEN
-CONJ_TAC THEN1 SRW_TAC [][mk_cat_mor,mk_cat_dom,mk_cat_obj] THEN
-CONJ_TAC THEN1 SRW_TAC [][mk_cat_mor,mk_cat_cod,mk_cat_obj] THEN
-CONJ_TAC THEN1 SRW_TAC [][mk_cat_obj,mk_cat_maps_to,mk_cat_id] THEN
-CONJ_TAC THEN1 (
-  SRW_TAC [][mk_cat_mor,mk_cat_id,mk_cat_dom] THEN
-  `composable c (f,c.id (c.dom f))` by (
-    FULL_SIMP_TAC (srw_ss()) [maps_to_def,composable_def] ) THEN
-  SRW_TAC [][mk_cat_comp] ) THEN
-CONJ_TAC THEN1 (
-  SRW_TAC [][mk_cat_mor,mk_cat_id,mk_cat_cod] THEN
-  `composable c (c.id (c.cod f),f)` by (
-    FULL_SIMP_TAC (srw_ss()) [maps_to_def,composable_def] ) THEN
-  SRW_TAC [][mk_cat_comp] ) THEN
-CONJ_TAC THEN1 (
-  SRW_TAC [][mk_cat_composable,mk_cat_comp] THEN
+`∀c. category_axioms c ⇒ is_category (mk_cat c)`,
+let fun sspecl l th = SIMP_RULE (srw_ss()) [] (Q.SPECL l th) in
+srw_tac [][is_category_def] >>
+fsrw_tac [][category_axioms_def] >>
+fsrw_tac [][sspecl [`c`,`(f,c.id(c.dom f))`,`c.dom f`] maps_to_dom_composable] >>
+fsrw_tac [][sspecl [`c`,`(c.id(c.cod f),f)`,`c.cod f`] maps_to_cod_composable] >>
+conj_tac  >- (
+  srw_tac [][] >>
   `composable c (c.comp (h,g),f)` by (
-    FULL_SIMP_TAC (srw_ss()) [composable_def,maps_to_def] ) THEN
+    fsrw_tac [][composable_def,maps_to_def] ) >>
   `composable c (h,c.comp (g,f))` by (
-    FULL_SIMP_TAC (srw_ss()) [composable_def,maps_to_def] ) THEN
-  SRW_TAC [][mk_cat_comp] ) THEN
-SRW_TAC [][mk_cat_maps_to] THEN
+    fsrw_tac [][composable_def,maps_to_def] ) >>
+  srw_tac [][] ) THEN
+srw_tac [][] >>
 `composable c (g,f)` by (
-  FULL_SIMP_TAC (srw_ss()) [composable_def,maps_to_def] ) THEN
-SRW_TAC [][mk_cat_comp] THEN
-FULL_SIMP_TAC (srw_ss()) [maps_to_def,composable_def])
+  fsrw_tac [][composable_def,maps_to_def] ) THEN
+fsrw_tac [][maps_to_def,composable_def] end)
+
+val composable_maps_to = Q.store_thm(
+"composable_maps_to",
+`∀c gf. is_category c ∧ composable c gf
+⇒ maps_to c (c.comp gf) (c.dom (SND gf)) (c.cod (FST gf))`,
+Cases_on `gf` >> srw_tac [][composable_def] >>
+fsrw_tac [][is_category_def,category_axioms_def] >>
+first_assum match_mp_tac >> srw_tac [][maps_to_def])
+
+val maps_to_composable = Q.store_thm(
+"maps_to_composable",
+`∀c gf x y z. maps_to c (SND gf) x y ∧ maps_to c (FST gf) y z
+⇒ composable c gf`,
+srw_tac [][composable_def,maps_to_def])
+
+val comp_mor_dom_cod = Q.store_thm(
+"comp_mor_dom_cod",
+`∀ c gf. is_category c ∧ composable c gf ⇒
+ (FST gf) ∈ c.mor ∧ (SND gf) ∈ c.mor ∧
+ (c.dom (c.comp gf) = c.dom (SND gf)) ∧
+ (c.cod (c.comp gf) = c.cod (FST gf))`,
+rpt strip_tac >>
+imp_res_tac composable_maps_to >>
+fsrw_tac [][maps_to_def,composable_def])
+
+val maps_to_obj = Q.store_thm(
+"maps_to_obj",
+`∀c f x y.
+is_category c ∧ maps_to c f x y
+⇒ x ∈ c.obj ∧ y ∈ c.obj`,
+srw_tac [][maps_to_def] >>
+fsrw_tac [][is_category_def,category_axioms_def])
+
+val id_inj = Q.store_thm(
+"id_inj",
+`∀c x y. is_category c ∧ x ∈ c.obj ∧ y ∈ c.obj ∧ (c.id x = c.id y)
+⇒ (x = y)`,
+srw_tac [][is_category_def,category_axioms_def] >>
+res_tac >> metis_tac [maps_to_def])
+
+val composable_comp = Q.store_thm(
+"composable_comp",
+`∀c f g h. is_category c ∧
+ composable c (g,f) ∧ composable c (h,g) ⇒
+ composable c (c.comp (h,g), f) ∧
+ composable c (h, c.comp (g,f))`,
+srw_tac [][] >>
+fsrw_tac [][is_category_def,category_axioms_def] >>
+fsrw_tac [][maps_to_def,composable_def])
+
+val id_mor = Q.store_thm(
+"id_mor",
+`∀c x. is_category c ∧
+ x ∈ c.obj ⇒
+ c.id x ∈ c.mor`,
+srw_tac [][is_category_def,category_axioms_def,maps_to_def])
+
+val id_composable_id = Q.store_thm(
+"id_composable_id",
+`∀c x. is_category c ∧
+ x ∈ c.obj ⇒
+ composable c (c.id x,c.id x)`,
+srw_tac [][] >>
+match_mp_tac maps_to_composable >>
+fsrw_tac [][is_category_def,category_axioms_def] >>
+metis_tac [])
+
+val left_right_inv_unique = Q.store_thm(
+"left_right_inv_unique",
+`∀c f g h. is_category c ∧
+ composable c (f,h) ∧ composable c (g,f) ∧
+ (c.comp (g,f) = c.id (c.dom f)) ∧
+ (c.comp (f,h) = c.id (c.cod f)) ⇒
+ (h = g)`,
+srw_tac [][is_category_def,category_axioms_def] >>
+`h ∈ c.mor ∧ g ∈ c.mor ∧
+ (c.dom f = c.cod h) ∧ (c.cod f = c.dom g)`
+   by fsrw_tac [][composable_def] >>
+metis_tac [composable_def])
+
+val id_dom_cod = Q.store_thm(
+"id_dom_cod",
+`∀c x. is_category c ∧ x ∈ c.obj ⇒
+ (c.dom (c.id x) = x) ∧
+ (c.cod (c.id x) = x)`,
+srw_tac [][is_category_def,category_axioms_def,maps_to_def])
+
+val id_comp_id = Q.store_thm(
+"id_comp_id",
+`∀c x. is_category c ∧ x ∈ c.obj ⇒
+ (c.comp (c.id x, c.id x) = c.id x)`,
+rpt strip_tac >>
+imp_res_tac id_dom_cod >>
+fsrw_tac [][is_category_def,category_axioms_def,maps_to_def] >>
+metis_tac [])
+
+val iso_pair_def = Define`
+  iso_pair c gf = composable c gf ∧
+    (c.comp gf = c.id (c.dom (SND gf))) ∧
+    (c.comp (SND gf, FST gf) = c.id (c.cod (SND gf)))`
+
+val iso_def = Define`
+  iso c f = ∃g. iso_pair c (g,f)`
+
+val iso_pair_sym = Q.store_thm(
+"iso_pair_sym",
+`is_category c ∧
+ iso_pair c (g,f) ⇒ iso_pair c (f,g)`,
+srw_tac [][is_category_def,category_axioms_def] >>
+fsrw_tac [][iso_pair_def,composable_def,maps_to_def] >>
+metis_tac [])
+
+val inv_unique = Q.store_thm(
+"inv_unique",
+`∀c f g h. is_category c ∧ iso_pair c (g,f) ∧ iso_pair c (h,f)
+⇒ (g = h)`,
+rpt strip_tac >>
+match_mp_tac left_right_inv_unique >>
+imp_res_tac iso_pair_sym >>
+fsrw_tac [][iso_pair_def] >>
+metis_tac [])
+
+val id_iso_pair = Q.store_thm(
+"id_iso_pair",
+`∀c x. is_category c ∧ x ∈ c.obj ⇒ iso_pair c (c.id x, c.id x)`,
+srw_tac [][iso_pair_def] >- (
+  match_mp_tac (GEN_ALL maps_to_composable) >>
+  fsrw_tac [][is_category_def,category_axioms_def] >>
+  metis_tac [] ) >>
+fsrw_tac [][is_category_def,category_axioms_def,maps_to_def] >>
+metis_tac [])
+
+val inv_def = Define`
+  inv c f = @g. iso_pair c (g,f)`
+
+val inv_elim_thm = Q.store_thm(
+"inv_elim_thm",
+`∀P (c:('a,'b) category) f g. is_category c ∧ iso_pair c (g,f) ∧ P g ⇒ P (inv c f)`,
+srw_tac [][inv_def] >>
+SELECT_ELIM_TAC >>
+srw_tac [SATISFY_ss][] >>
+qsuff_tac `x=g` >- srw_tac [][] >>
+match_mp_tac inv_unique >>
+fsrw_tac [SATISFY_ss][]);
+
+fun is_inv tm = let
+  val (f,_) = dest_comb tm
+  val (f,_) = dest_comb f
+  val ("inv",ty) = dest_const f
+in
+  can (match_type ``:('a,'b) category -> 'b -> 'b``) ty
+end handle HOL_ERR _ => false | Bind => false
+
+fun inv_elim_tac (g as (_, w)) = let
+  val t = find_term is_inv w
+in
+  CONV_TAC (UNBETA_CONV t) THEN
+  MATCH_MP_TAC inv_elim_thm THEN BETA_TAC
+end g
+
+val inv_eq_iso_pair = Q.store_thm(
+"inv_eq_iso_pair",
+`∀c f g. is_category c ∧ iso_pair c (g,f) ⇒ (inv c f = g)`,
+srw_tac [][] >>
+inv_elim_tac >>
+srw_tac [][])
+
+val inv_idem = Q.store_thm(
+"inv_idem",
+`∀c f. is_category c ∧
+ iso c f ⇒
+ iso c (inv c f) ∧ (inv c (inv c f) = f)`,
+srw_tac [][iso_def] >>
+inv_elim_tac >>
+srw_tac [][] >>
+TRY inv_elim_tac >>
+metis_tac [iso_pair_sym])
+
+val iso_pair_mor = Q.store_thm(
+"iso_pair_mor",
+`∀c gf. is_category c ∧
+ iso_pair c gf ⇒
+ (FST gf) ∈ c.mor ∧ (SND gf) ∈ c.mor`,
+srw_tac [][iso_pair_def,composable_def])
+
+val iso_mor = Q.store_thm(
+"iso_mor",
+`∀c f. is_category c ∧ iso c f
+⇒ f ∈ c.mor`,
+srw_tac [][iso_def] >>
+imp_res_tac iso_pair_mor >>
+fsrw_tac [][])
+
+val inv_mor_dom_cod = Q.store_thm(
+"inv_mor_dom_cod",
+`∀c f. is_category c ∧
+ iso c f ⇒
+ (inv c f) ∈ c.mor ∧
+ (c.dom (inv c f) = c.cod f) ∧
+ (c.cod (inv c f) = c.dom f)`,
+srw_tac [][iso_def] >>
+imp_res_tac inv_eq_iso_pair >>
+imp_res_tac iso_pair_mor >>
+imp_res_tac iso_pair_sym >>
+fsrw_tac [][iso_pair_def,composable_def])
+
+val inv_composable = Q.store_thm(
+"inv_composable",
+`∀c f. is_category c ∧ iso c f ⇒
+ composable c (f, inv c f) ∧
+ composable c (inv c f, f)`,
+srw_tac [][iso_def] >>
+imp_res_tac iso_pair_sym >>
+match_mp_tac maps_to_composable >>
+imp_res_tac inv_eq_iso_pair >>
+fsrw_tac [][iso_pair_def] >>
+srw_tac [][maps_to_def] >>
+fsrw_tac [][composable_def])
+
+val comp_inv_id = Q.store_thm(
+"comp_inv_id",
+`∀c f. is_category c ∧ iso c f ⇒
+ (c.comp (f, inv c f) = c.id (c.cod f)) ∧
+ (c.comp (inv c f, f) = c.id (c.dom f))`,
+srw_tac [][iso_def] >>
+inv_elim_tac >>
+imp_res_tac iso_pair_sym >>
+imp_res_tac iso_pair_def >>
+fsrw_tac [][composable_def] >>
+metis_tac [])
+
+val invs_composable = Q.store_thm(
+"invs_composable",
+`∀c gf. is_category c ∧ composable c gf ∧
+ iso c (FST gf) ∧ iso c (SND gf) ⇒
+ composable c (inv c (SND gf), inv c (FST gf))`,
+srw_tac [][] >>
+imp_res_tac inv_mor_dom_cod >>
+fsrw_tac [][composable_def])
+
+val iso_pair_comp = Q.store_thm(
+"iso_pair_comp",
+`∀c gf. is_category c ∧ composable c gf ∧
+ iso c (FST gf) ∧ iso c (SND gf) ⇒
+ iso_pair c (c.comp gf, c.comp (inv c (SND gf), inv c (FST gf)))`,
+srw_tac [][] >>
+`composable c (inv c (SND gf), inv c (FST gf))` by imp_res_tac invs_composable >>
+`composable c (c.comp gf, c.comp (inv c (SND gf), inv c (FST gf)))` by (
+  match_mp_tac maps_to_composable >> srw_tac [][] >>
+  imp_res_tac composable_maps_to >>
+  imp_res_tac inv_mor_dom_cod >>
+  imp_res_tac comp_mor_dom_cod >>
+  map_every qexists_tac [`c.cod (FST gf)`,`c.dom (SND gf)`,`c.cod (FST gf)`] >>
+  srw_tac [][] >> fsrw_tac [][maps_to_def] ) >>
+Cases_on `gf` >> fsrw_tac [][] >>
+qmatch_assum_rename_tac `composable c (inv c f,inv c g)` [] >>
+imp_res_tac is_category_def >>
+`c.comp (c.comp (g,f),c.comp(inv c f,inv c g)) = c.comp (c.comp (c.comp (g,f), inv c f), inv c g)` by (
+  fsrw_tac [][category_axioms_def] >>
+  first_assum match_mp_tac >> srw_tac [][] >>
+  match_mp_tac (DISCH_ALL (CONJUNCT1 (UNDISCH_ALL (SPEC_ALL composable_comp)))) >>
+  fsrw_tac [][inv_composable] ) >>
+`c.comp (c.comp (g,f), inv c f) = c.comp (g, c.comp (f, inv c f))` by (
+  fsrw_tac [][category_axioms_def] >>
+  first_assum (match_mp_tac o GSYM) >> srw_tac [][] >>
+  fsrw_tac [][inv_composable] ) >>
+`c.comp (c.comp (inv c f, inv c g), c.comp (g,f)) = c.comp (inv c f, c.comp (inv c g, c.comp (g,f)))` by (
+  fsrw_tac [][category_axioms_def] >>
+  first_assum (match_mp_tac o GSYM) >> srw_tac [][] >>
+  match_mp_tac (DISCH_ALL (CONJUNCT2 (UNDISCH_ALL (SPEC_ALL composable_comp)))) >>
+  fsrw_tac [][inv_composable] ) >>
+`c.comp (inv c g, c.comp (g,f)) = c.comp (c.comp (inv c g, g), f)` by (
+  fsrw_tac [][category_axioms_def] >>
+  first_assum match_mp_tac >> srw_tac [][] >>
+  fsrw_tac [][inv_composable] ) >>
+`c.cod f = c.dom g` by fsrw_tac [][composable_def] >>
+imp_res_tac comp_inv_id >>
+imp_res_tac inv_mor_dom_cod >>
+imp_res_tac comp_mor_dom_cod >>
+fsrw_tac [][] >>
+fsrw_tac [][category_axioms_def] >>
+srw_tac [][iso_pair_def] >>
+metis_tac [])
+
+val iso_objs_def = Define`
+  iso_objs c a b = ∃f. maps_to c f a b ∧ iso c f`
+
+val unit_cat_def = Define`
+  unit_cat = mk_cat <| obj := {()}; mor := {()}; dom := K (); cod := K (); id := K (); comp := K () |>`
+
+val is_category_unit_cat = Q.store_thm(
+"is_category_unit_cat",
+`is_category unit_cat`,
+srw_tac [][unit_cat_def] >>
+match_mp_tac mk_cat_is_category >>
+srw_tac [][category_axioms_def,maps_to_def])
+
+val op_cat_def = Define`
+  op_cat c = <| obj := c.obj; mor := c.mor; dom := c.cod; cod := c.dom; id := c.id; comp := λ(f,g). c.comp (g,f) |>`
+
+val op_cat_idem = Q.store_thm(
+"op_cat_idem",
+`op_cat (op_cat c) = c`,
+srw_tac [][op_cat_def,category_component_equality,
+           FUN_EQ_THM,pairTheory.UNCURRY])
+
+val op_cat_axioms = Q.store_thm(
+"op_cat_axioms",
+`category_axioms c ⇒ category_axioms (op_cat c)`,
+srw_tac [][category_axioms_def,op_cat_def,maps_to_def,composable_def])
+
+val op_cat_extensional = Q.store_thm(
+"op_cat_extensional",
+`extensional_category c ⇒ extensional_category (op_cat c)`,
+srw_tac [][extensional_category_def,op_cat_def] >>
+srw_tac [][extensional_def,IN_DEF,pairTheory.UNCURRY] >>
+fsrw_tac [][composable_def,IN_DEF,extensional_def])
+
+val is_category_op_cat = Q.store_thm(
+"is_category_op_cat",
+`is_category c ⇒ is_category (op_cat c)`,
+srw_tac [][is_category_def,op_cat_axioms,op_cat_extensional])
+
+val op_maps_to = Q.store_thm(
+"op_maps_to",
+`maps_to c f x y ⇒ maps_to (op_cat c) f y x`,
+srw_tac [][maps_to_def,op_cat_def])
+
+val op_composable = Q.store_thm(
+"op_composable",
+`composable c (SND gf, FST gf) ⇒ composable (op_cat c) gf`,
+srw_tac [][composable_def,op_cat_def])
 
 val _ = export_theory ()
